intermediate lemmas

src/Verification.v
@@ -12,6 +12,15 @@ Module Verification.
 Definition eval := Language.semantics.
 Definition eval' := Assembly.semantics.
 
+Theorem comp_newstate :
+  forall p q, Compiler.compile p q ->
+              q.(Assembly.pc) = Compiler.new_pc (p.(Language.prog)) (p.(Language.pc)) /\
+              q.(Assembly.ac) = p.(Language.ptr) /\
+              q.(Assembly.mem) = p.(Language.mem) /\
+              q.(Assembly.b) = 0.
+Proof.
+Admitted.
+
 Theorem match_preserve : 
   forall p p', Language.semantics p p' ->
                Compiler.matched (Language.prog p) ->
@@ -19,6 +28,43 @@ Theorem match_preserve :
 Proof.
 Admitted.
 
+Definition first_comp_instr (i : Language.instr) : Assembly.instr :=
+  match i with
+  | Language.PtrInc => Assembly.Add 1
+  | Language.PtrDec => Assembly.Sub 1
+  | Language.Inc => Assembly.Swap
+  | Language.Dec => Assembly.Swap
+  | Language.Jump => Assembly.Skip
+  | Language.Ret => Assembly.Skip
+  | Language.Halt => Assembly.Halt
+  end.
+
+Theorem first_instr_comp : forall p q i, Compiler.compile p q ->
+                           Language.read_instr p i ->
+                           Assembly.read_instr q (first_comp_instr i).
+Proof.
+Admitted.
+
+Theorem sequence_comp_ptrinc :
+  forall p p' q, Compiler.compile p q -> eval p p' ->
+              Language.read_instr p Language.PtrInc ->
+              exists q', (eval' q q' /\ Assembly.read_instr q' 
+              (first_comp_instr (Language.read_instr' p'.(Language.prog) p'.(Language.pc)))).   
+Proof.
+Admitted.
+Theorem sequence_comp_inc :
+  forall p p' q, Compiler.compile p q -> eval p p' ->
+              Language.read_instr p Language.Inc ->
+              exists q'1, (eval' q q'1 /\ Assembly.read_instr q'1 Assembly.Swap) /\
+              exists q'2, (eval' q'1 q'2 /\ Assembly.read_instr q'2 Assembly.Load) /\
+              exists q'3, (eval' q'2 q'3 /\ Assembly.read_instr q'3 (Assembly.Add 1)) /\
+              exists q'4, (eval' q'3 q'4 /\ Assembly.read_instr q'4 Assembly.Store) /\
+              exists q'5, (eval' q'4 q'5 /\ Assembly.read_instr q'5 Assembly.Zero) /\
+              exists q'6, (eval' q'5 q'6 /\ Assembly.read_instr q'6 Assembly.Swap) /\
+              exists q', (eval' q'6 q' /\ Assembly.read_instr q'
+              (first_comp_instr (Language.read_instr' p'.(Language.prog) p'.(Language.pc)))).   
+Proof.
+Admitted.
 Theorem comp_correct : 
   Simulation.plus_forward_sim Compiler.compile eval eval'.
 Proof.
@@ -38,7 +84,37 @@ Proof.
       reflexivity.
     + inversion compileH.
       remember (Compiler.compile' p') as q'.
-      assert (Assembly.read_instr q (Assembly.Add 1)).
+      assert (q.(Assembly.pc) = Compiler.new_pc (p.(Language.prog)) (p.(Language.pc)) /\
+              q.(Assembly.ac) = p.(Language.ptr) /\
+              q.(Assembly.mem) = p.(Language.mem) /\
+              q.(Assembly.b) = 0).
+      apply comp_newstate.
+      assumption.
+      assert (q'.(Assembly.pc) = Compiler.new_pc (p'.(Language.prog)) (p'.(Language.pc)) /\
+              q'.(Assembly.ac) = p'.(Language.ptr) /\
+              q'.(Assembly.mem) = p'.(Language.mem) /\
+              q'.(Assembly.b) = 0).
+      {  
+        apply comp_newstate.
+        apply Compiler.comp_r. 
+        assumption.
+        assumption.
+      }
+      destruct H7. destruct H9. destruct H10.
+      destruct H8. destruct H12. destruct H13.
+      assert (Assembly.read_instr q' (first_comp_instr
+               (Language.read_instr' p'.(Language.prog) p'.(Language.pc)))).
+      {
+        apply first_instr_comp with (p := p').
+        apply Compiler.comp_r.
+        assumption.
+        assumption.
+        apply Language.ri.
+        reflexivity.
+      }
+      remember ((first_comp_instr (Language.read_instr'
+               (Language.prog p') (Language.pc p')))) as i.
+      
       (* todo: prove sufficient conditions 
                for eval'+ q q' to hold, instead of the stronger eval' q q'*)
       
